Proof for updating local ephemeral proposal when backup gets ApplyAsBackup RPC;
this is a bit of a "bogus" proof in the sense that backup servers don't
even use the ephemeral proposal. But, if we encoded this fact in the
invariants, then we would need to break the existing own_primary_ghost
abstraction and would need to give as precondition to ApplyAsBackup
a witness that says the server is not primary in that epoch.

I decided to just do the bogus proof instead (unclear if this is
actually less work).

src/program_proof/simplepb/pb_definitions.v
@@ -440,7 +440,7 @@ Definition own_Server (s:loc) γ γsrv γeph own_StateMachine mu : iProp Σ :=
   (* ghost-state *)
   "Heph" ∷ own_ephemeral_proposal γeph epoch opsfull_ephemeral ∗
   "Heph_unused" ∷ own_unused_ephemeral_proposals γeph epoch ∗
-  "Heph_prop_lb" ∷ (if isPrimary then True else is_proposal_lb γ epoch opsfull_ephemeral) ∗
+  "#Heph_prop_lb" ∷ □(if isPrimary then True else is_proposal_lb γ epoch opsfull_ephemeral) ∗
   "Hstate" ∷ own_StateMachine epoch ops sealed (own_Server_ghost γ γsrv γeph) ∗
   "%Hσ_nextIndex" ∷ ⌜length ops = int.nat nextIndex⌝ ∗
   "%Heph_proposal" ∷ ⌜ True ⌝ (* opsfull_eph has `nextRoIndex` RO ops as its tail. *) ∗
@@ -459,7 +459,7 @@ Definition own_Server (s:loc) γ γsrv γeph own_StateMachine mu : iProp Σ :=
   "#HopAppliedConds_conds" ∷ ([∗ map] i ↦ cond ∈ opAppliedConds, is_cond cond mu) ∗
 
   (* primary-only *)
-  "HprimaryOnly" ∷ if isPrimary then (
+  "#HprimaryOnly" ∷ □ if isPrimary then (
             ∃ (clerkss:list Slice.t) (backups:list pb_server_names),
             (* Because the state machine is async, we might not have "is_tok"
                right when we become leader, but we will definitely have a fupd
